---
title: 'Part III: Invariance of Natural-Gradients'
date: 2021-11-02
permalink: /posts/2021/11/Geomopt03/
tags:
  - Natural Gradient Descent
  - Information Geometry
  - Riemannian Manifold
---


Goal
------
This blog post should help readers to understand the invariance of natural-gradients.
We will also discuss why the Euclidean steepest direction is NOT invariant.

We will give an informal introduction with a focus on high level of ideas.




# Parameter Transformation and Invariance
------
In [Part II]({{ site.baseurl }}{% post_url 2021-10-04-Geomopt02 %}#riemannian-gradients-as-tangent-vectors-optional), we have shown that a Riemannian gradient is a parametric representation of the tangent direction of a curve in a  manifold.
Since a curve and its tangent direction are geometric obejects, they should be invariant to the choice of parametrization.
In other words, geometric properties should be persevered in any valid coordinate system. This is a coordinate-free argument. 

The argument could be abstract for beginners. To be more concrete, we consider the corresponding coordinate-dependent argument: geometric properties should remain unchanged if we perform a (valid) parameter transformation. This coordinate-dependent argument also gives us a rule to compute natrual-gradients under a parameter transformation.

The transformation rules are summarized in the following table

|   Type of  directions  |   transformation rules  |
|:------------|:-------------:|
| Euclidean gradient |  `$\eqref{6}$`  | 
| Euclidean steepest descent direction (normalized Euclidean gradient)  |  N/A  |   
| Riemannian gradient |  `$\eqref{7}$` | 
|  Riemannian steepest descent direction (normalized Riemannian gradient) |  `$\eqref{7}$`  |   

The following example illustrates these transformation rules. 
<div class="notice--info" markdown="1">
<details>
<summary>Univariate Gaussian example: (click to expand)</summary>
<fieldset class="field-set" markdown="1">
> Consider the following scalar function
> `$$
> \begin{aligned}
> h_\tau(\tau):= E_{q(w|\tau)} [ w^2 + \log q(w|\tau) ]
> = \mu^2 + \frac{1}{s} + \frac{1}{2} \log(s)- \frac{1}{2}(1+\log(2\pi))
> \end{aligned}
> $$`
> where  `$q(w|\tau)= \mathcal{N}(w|\mu,s^{-1})$` is a Gaussian family with mean `$\mu$`, variance `$s^{-1}$`, 
>   intrinsic parametrization `$\tau=(\mu,s)$`, and parameter space `$\Omega_\tau=\{(\mu,s)|\mu \in \mathcal{R},s>0 \}$`.
>
> The FIM of Gaussian $q(w|\tau)$ under parametrization `$\tau$` is
> `$$
> \begin{aligned}
> \mathbf{F}_\tau (\tau) := -E_{q(w|\tau)} [ \nabla_\tau^2 \log q(w|\tau) ] 
> =
>\begin{bmatrix}
>s & 0 \\
>0 & \frac{1}{2s^2}
>\end{bmatrix}
> \end{aligned}
> $$`
> We consider a member $\tau_0=(0.5,0.5)$ in the Gaussian family.
> The Euclidean gradient is 
>`$$
> \begin{aligned}
> \mathbf{g}_\tau (\tau_0) :=
> \nabla_\tau h_\tau(\tau_0) =
>\begin{bmatrix}
>2 \mu \\
>-\frac{1}{s^2} +\frac{1}{2s}
>\end{bmatrix}_{\tau=\tau_0}
>=\begin{bmatrix}
>1 \\ -3
>\end{bmatrix}
> \end{aligned}
>$$`
> The natural/Riemannian gradient is 
>`$$
> \begin{aligned}
> \hat{\mathbf{g}}_\tau (\tau_0) :=
> \mathbf{F}_\tau^{-1} (\tau_0) \nabla_\tau h_\tau(\tau_0) =
>\begin{bmatrix}
>2 \mu s^{-1}  \\
>( -\frac{1}{s^2} +\frac{1}{2s} ) (2s^2)
>\end{bmatrix}_{\tau=\tau_0}
>=\begin{bmatrix}
>2 \\ -\frac{3}{2}
>\end{bmatrix}
> \end{aligned}
>$$`
>
> Now, consider the following re-parametrization of the function
>
> `$$
> \begin{aligned}
> h_\lambda(\lambda)= E_{q(w|\lambda)} [ w^2 + \log q(w|\lambda)]
> = \mu^2 + v - \frac{1}{2} \log(v) - \frac{1}{2}(1+\log(2\pi))
> \end{aligned}
> $$`
> where `$q(w|\lambda)= \mathcal{N}(w|\mu,v)$` with mean `$\mu$` and variance `$v=s^{-1}$`,
>   intrinsic parametrization `$\lambda=(\mu,v)$`, and parameter space `$\Omega_\lambda=\{(\mu,v)|\mu \in \mathcal{R},v>0 \}$`.
>
> The FIM of Gaussian $q(w|\lambda)$ under parametrization `$\lambda$` is
> `$$
> \begin{aligned}
> \mathbf{F}_\lambda (\lambda):= -E_{q(w|\lambda)} [ \nabla_\lambda^2 \log q(w|\lambda) ] 
> =
>\begin{bmatrix}
>\frac{1}{v} & 0 \\
>0 & \frac{1}{2v^2}
>\end{bmatrix}
> \end{aligned}
> $$`
> 
> The Jacobian matrix is
> `$$
> \begin{aligned}
> \mathbf{J} :=\frac{\partial \lambda(\tau)}{\partial \tau} = 
>\begin{bmatrix}
> 1 & 0 \\
>0 & -\frac{1}{s^2}
>\end{bmatrix}
> \end{aligned}
> $$` where $\lambda(\tau)=(\mu,v)=(\mu,\frac{1}{s})$ and $\tau=(\mu,s)$.
>
> We can verify that `$\eqref{8}$` holds for the FIM.
>
> Consider the same member $\lambda_0=(0.5,2)$ in the Gaussian family.
> The Euclidean gradient is 
>`$$
> \begin{aligned}
> \mathbf{g}_\lambda (\lambda_0) :=
> \nabla_\lambda h_\lambda(\lambda_0) =
>\begin{bmatrix}
>2 \mu \\
>1 - \frac{1}{2v}
>\end{bmatrix}_{\lambda=\lambda_0}
>=\begin{bmatrix}
>1 \\ \frac{3}{4}
>\end{bmatrix} 
> \end{aligned}
>$$`
> We can verify that `$\eqref{6}$` holds for the Euclidean gradient.
>
> The natural/Riemannian gradient is 
>`$$
> \begin{aligned}
> \hat{\mathbf{g}}_\lambda (\lambda_0) :=
> \mathbf{F}_\lambda^{-1} (\lambda_0) \nabla_\lambda h_\lambda(\lambda_0) =
>\begin{bmatrix}
>2 \mu  v \\
>( 1 - \frac{1}{2v} ) (2v^2)
>\end{bmatrix}_{\lambda=\lambda_0}
>=\begin{bmatrix}
>2 \\ 6
>\end{bmatrix}
> \end{aligned}
>$$`
>
> We can verify that `$\eqref{7}$` holds for the Riemannian gradient
</fieldset>
</details>
</div>


<div class="notice--success" markdown="1">
We will show that two key **geometric properties** remains the same under any **intrinsic** parameter transformation.
1. Directional derivative 
2. Length of a Riemannian vector/gradient induced by the Fisher-Rao metric
</div>

Thanks to these properties, we will show that the optimal solution of the [Riemannian steepest direction]({{ site.baseurl }}{% post_url 2021-10-04-Geomopt02 %}#riemannian-steepest-direction) considered in Part II is equivalent under an intrinsic parameter transformation. This is in contrast with the Euclidean steepest direction which is not invaraint under an intrinsic parameter transformation.


In [Part II]({{ site.baseurl }}{% post_url 2021-10-04-Geomopt02 %}#riemannian-gradients-as-tangent-vectors-optional), we consider a point $\mathbf{x}_0$ in a manifold $\mathcal{M}$, a (1-dimensional) curve $\gamma(t)$, and a smooth scalar function $h: \mathcal{M} \to \mathcal{R}$.
Given an intrinsic parametrization $\tau$ containing the point, we consider the following parametric representations.
 
|   geometric object   |   parametric representation  |
|:------------|:-------------:|
| point `$\mathbf{x}_0$` |  `$\tau_0$`   | 
| curve  `$\gamma(t)$`  | `$\gamma_\tau(t) $`  | 
| function  `$h(x_0)$`  | `$h_\tau(\tau_0) $`  |   




## Transformation Rules for Natural Gradients and Euclidean Gradients 

Intuitively, the following identity should hold for any two (intrinsic) parametrizations $\tau$ and $\lambda$.
`$$
\begin{aligned}
h(\gamma(t)) = h_\tau(\gamma_\tau(t)) = h_\lambda(\gamma_\lambda(t))
\end{aligned}
$$` where we consider $t$ to be fixed. 

Technically speaking,  domain `$\mathbf{I}_\tau$` of curve `$\gamma_\tau(t)$` and  domain `$\mathbf{I}_\lambda$` of curve `$\gamma_\lambda(t)$` may be different.
For simplicity, we assume both domains are open intervals containing 0.
In other words, `$\gamma_\tau(0)=\tau_0$` and `$\gamma_\lambda(0)=\lambda_0$`  are parametric representations of the same point `$\mathbf{x}_0$`.


From the above expression, we can see that directional derivatives should be the same at $t=0$
`$$
\begin{aligned}
 \frac{d h_\tau({\gamma}_\tau(t)) }{d t} \Big|_{t=0} = \frac{d h_\lambda({\gamma}_\lambda(t)) }{d t} \Big|_{t=0} 
\end{aligned}\tag{1}\label{1}
$$`

In [Part II]({{ site.baseurl }}{% post_url 2021-10-04-Geomopt02 %}#riemannian-gradients-as-tangent-vectors-optional), we have shown that 
`$$
\begin{aligned}
 \frac{d h_\tau({\gamma}_\tau(t)) }{d t} \Big|_{t=0} &=  [\nabla h_\tau(\mathbf{\tau}_0)  ]^T  \frac{d {\gamma}_\tau(t) }{d t} \Big|_{t=0}   \\ 
 \frac{d h_\lambda({\gamma}_\lambda(t)) }{d t} \Big|_{t=0} & = [\nabla h_\lambda(\mathbf{\lambda}_0) ]^T  \frac{d {\gamma}_\lambda(t) }{d t} \Big|_{t=0}  
\end{aligned}
$$` where $\nabla$ is the standard (coordinate) derivative.


Recall that in [Part II]({{ site.baseurl }}{% post_url 2021-10-04-Geomopt02 %}#riemannian-gradients-as-tangent-vectors-optional),  we have shown that `$\frac{d {\gamma}_\tau(t) }{d t} \Big|_{t=0}$` is a  parametric representation of a tangent vector, which is a Riemannian gradient.
Notice that `$\nabla h_\lambda(\mathbf{\lambda}_0)$` is a Euclidean gradient[^1]. 

We will use the following notations to simplify expressions.

|  Notations   |   Meanings  |
|:------------|:-------------:|
| Euclidean gradient `$(g_\tau)_i$`  |  $i$-th entry  under parametrization $\tau$  | 
| Riemannian gradient `$(\hat{g}_\tau)^j$` |  $j$-th entry under parametrization $\tau$  | 
| Parameter `$\tau^j$` |  $j$-th parameter under parametrization   $\tau$  | 
   
Using these notations, the derivational derivatives then can be re-expressed as

`$$
\begin{aligned}
 \frac{d h_\tau({\gamma}_\tau(t)) }{d t} \Big|_{t=0} &= \sum_{i}  (g_\tau)_i  (\hat{g}_\tau)^i  = \mathbf{g}_\tau^T \hat{\mathbf{g}}_\tau \\ 
 \frac{d h_\lambda({\gamma}_\lambda(t)) }{d t} \Big|_{t=0} & =\sum_{i}  (g_\lambda)_i (\hat{g}_\lambda)^i =  {\mathbf{g}}_\lambda^T \hat{\mathbf{g}}_\lambda
\end{aligned}\tag{2}\label{2}
$$`
where  `$\mathbf{g}_\lambda$` and `$\mathbf{g}_\tau$` are Euclidean gradients (e.g.,  `$\mathbf{g}_\tau=\nabla h_\tau(\tau_0) $`)  while  `$\hat{\mathbf{g}}_\lambda$` and `$\hat{\mathbf{g}}_\tau$`  are  Riemannian gradients (e.g., `$\hat{\mathbf{g}}_\tau=\frac{d \gamma_\tau(0) }{d t}$`) .



By `$\eqref{1}$` and `$\eqref{2}$`, we have the following identity obtained from the **geometric property** of directional derivatives.
`$$
\begin{aligned}
 \mathbf{g}_\tau^T \hat{\mathbf{g}}_\tau  =  \mathbf{g}_\lambda^T \hat{\mathbf{g}}_\lambda 
\end{aligned}\tag{3}\label{3}
$$`


Now, we discuss the parameter transformation between $\tau$ and $\lambda$, where we can express $\lambda$ in terms of $\tau$ denoted by $\lambda(\tau)$.


By the (standard) chain rule for a Euclidean gradient[^2], we has
`$$
\begin{aligned}
(g_\tau)_i = \sum_{k}  \color{red}{ (g_\lambda)_k} \frac{\color{red}{ \partial \lambda^k(\tau) }}{ \partial \tau^i } 
\end{aligned}
\tag{4}\label{4}
$$` 


Let `$J_{ki}:=\frac{\partial \lambda^k(\tau) }{ \partial \tau^i }$` denotes the $(k,i)$ entry of the Jacobian matrix. We illustrate our matrix notation in a 2D case as below.

`$$
\begin{aligned}
\begin{matrix}
& \\
\mathbf{J} = 
    \left ( \vphantom{ \begin{matrix} 12 \\ 12  \end{matrix} } \right .
\end{matrix}
\hspace{-1.2em}
\begin{matrix}
    i=1 & i=2 \\ \hline
    J_{11} & J_{12}  \\
   J_{21} & J_{22} \\
\end{matrix}
\hspace{-0.2em}
\begin{matrix}
& \\
\left . \vphantom{ \begin{matrix} 12 \\ 12  \end{matrix} } \right )
    \begin{matrix}
    k=1 \\ k=2 
    \end{matrix}
\end{matrix}
\end{aligned}\tag{5}\label{5}
$$`

Eq. `$\eqref{4}$` gives us the transformation rule for Eulcidean gradients (denoted by a row vector)  as below in a vector form.

<div class="notice--success" markdown="1">
`$$
\begin{aligned}
\mathbf{g}_\tau^T =  \mathbf{g}_\lambda^T \mathbf{J}
\end{aligned}\tag{6}\label{6},
$$`

Note:
<span style="color:blue">**row**</span> vector `${\mathbf{g}}_\tau^T$` can be computed via a vector-Jacobian product in any standard Auto-Diff toolbox given that `${\mathbf{g}}_\lambda$` is pre-computed.
</div>


By Eq `$\eqref{3}$`, we obtain the transformation rule for Riemannian gradients  (denoted by a column vector) as below,  where `$\mathbf{Q}:=\mathbf{J}^{-1}$` is also a Jacobian matrix and `$Q_{ki}=\frac{\partial \tau^k(\lambda)}{\partial \lambda^i}$` is the `$(k,i)$` entry of matrix `$\mathbf{Q}$`.

<div class="notice--success" markdown="1">
`$$
\begin{aligned}
\hat{\mathbf{g}}_\tau= \mathbf{J}^{-1}  \hat{\mathbf{g}}_\lambda 
\end{aligned}\tag{7}\label{7}
$$`

Note:
<span style="color:blue">**column**</span> vector `$\hat{\mathbf{g}}_\tau$` can be computed via a Jacobian-vector product used in forward-mode differentiation  {% cite lin2021tractable %} {% cite salimbeni2018natural %} given that `$\hat{\mathbf{g}}_\lambda$` is pre-computed.
</div>

The elementwise expression of the transformation rule for Riemannian gradients is
`$$
\begin{aligned}
(g_\tau)^k
 = \sum_{i}  \frac{ \partial \tau^k(\lambda)  }{\color{red} {\partial  \lambda^i} }  \color{red} {(g_\lambda)^i}
\end{aligned},
$$` 

Note that these transformation rules are valid  when the Jacobian matrix `$\mathbf{J}$` is square and non-singular.
As we discussed in Part I about [intrinsic parameterizations]({{ site.baseurl }}{% post_url 2021-09-06-Geomopt01 %}#intrinsic-parameterizations), the transformation map between $\tau$ and $\lambda$ must be bi-jective, which implies the Jacoabian matrix is square. 
Moreover, the map and its inverse map should be smooth, which implies that the Jacobian matrix is well-defined and non-singular.


## Transformation Rule for the Fisher Information Matrix

Now, we discuss a transformation rule for the Fisher information matrix (FIM) as defined at [Part I]({{ site.baseurl }}{% post_url 2021-09-06-Geomopt01 %}#fisher-rao-metric).

`$$
\begin{aligned}
 F_{ij}(\tau) := E_{p(w|\tau) }  [ \Big( \partial_{\tau_i} \log p(w|\tau ) \Big)  \Big(\partial_{\tau_j} \log p(w|\tau) \Big) ]
\end{aligned}
$$`
Since $ \log p(w|\tau )$ can be considered as a scalar function $h$ defined on the manifold for any valid $w$, we have 
`$$
\begin{aligned}
 \log p(w|\tau_0  ) = h_\tau(\tau_0) = h_\lambda(\lambda_0) =  \log p(w|\lambda_0  )
\end{aligned}
$$`

Thus, the FIM can be computed as
`$$
\begin{aligned}
 F_{ij}(\tau_0) &= E_{p(w|\tau_0) }  [ \Big( \partial_{\tau_i} \log p(w|\tau_0 ) \Big)  \Big(\partial_{\tau_j} \log p(w|\tau_0) \Big) ] \\
&=  E_{p(w|\lambda_0) }  [ \Big( \partial_{\tau_i} \log p(w|\tau_0 ) \Big)  \Big(\partial_{\tau_j} \log p(w|\tau_0) \Big) ]\\
\end{aligned}
$$`

Recall that by the standard chain rule, we have 
`$$
\begin{aligned}
\partial_{\tau_i} \log p(w|\tau_0 ) = \sum_k \frac{ \partial \lambda^k(\tau_0) }{ \partial \tau^i } \Big( \partial_{\lambda_k} \log p(w|\lambda_0 ) \Big)
\end{aligned}
$$`
 
Moreover, the Jacobian matrix does not depent on $w$. Therefore, we have
`$$
\begin{aligned}
 F_{ij}(\tau_0) 
&=  E_{p(w|\lambda_0) }  [ \Big( \partial_{\tau_i} \log p(w|\tau_0 ) \Big)  \Big(\partial_{\tau_j} \log p (w|\tau_0) \Big) ]\\
&=  E_{p(w|\lambda_0) }  [ \Big( \sum_k \frac{ \partial \lambda^k(\tau_0) }{ \partial \tau^i } \partial_{\lambda_k} \log p(w|\lambda_0 ) \Big)  \Big(  \sum_l \frac{ \partial \lambda^l(\tau_0) }{ \partial \tau^j } \partial_{\lambda_l} \log p(w|\lambda_0 ) \Big) ] \\
&= \sum_k \sum_l  \frac{ \partial \lambda^k(\tau_0) }{ \partial \tau^i }  \frac{ \partial \lambda^l(\tau_0) }{ \partial \tau^j }  E_{p(w|\lambda_0) }  [ \Big(  \partial_{\lambda_k} \log p(w|\lambda_0 ) \Big)  \Big(  \partial_{\lambda_l} \log p(w|\lambda_0 ) \Big) ] \\
&= \sum_k \sum_l  \frac{ \partial \lambda^k(\tau_0) }{ \partial \tau^i }  \frac{ \partial \lambda^l(\tau_0) }{ \partial \tau^j } F_{kl}(\lambda_0)
\end{aligned}
$$`

We can re-express the above expression in a matrix form as below. This is the transformation rule for the FIM.

<div class="notice--success" markdown="1">
`$$
\begin{aligned}
\mathbf{F}_{\tau} (\tau_0) = \underbrace{\mathbf{J}^T}_{  \frac{ \partial \lambda^i(\tau_0) }{ \partial \tau^k }  } \mathbf{F}_{\lambda} (\lambda_0) \underbrace{\mathbf{J}}_{  \frac{ \partial \lambda^l(\tau_0) }{ \partial \tau^j }  } 
\end{aligned}\tag{8}\label{8}
$$`
</div>

By using this transformation rule, we can show that another **geometric property**: the length of a Riemannian vector is preserved.

We can see that the length of a Riemannian vector is also invariant.
`$$
\begin{aligned}
\| \hat{\mathbf{g}}_\tau \|^2_{F_{\tau_0}} &= [\hat{\mathbf{g}}_\tau]^T \mathbf{F}_{\tau} (\tau_0) \hat{\mathbf{g}}_\tau \\
&= [\mathbf{J}^{-1} \hat{\mathbf{g}}_\lambda]^T \mathbf{F}_{\tau} (\tau_0) \mathbf{J}^{-1} \hat{\mathbf{g}}_\lambda \\
&= [\hat{\mathbf{g}}_\lambda]^T [ \mathbf{J}^{-T}  \mathbf{F}_{\tau} (\tau_0) \mathbf{J}^{-1} ] \hat{\mathbf{g}}_\lambda \\
&= [\hat{\mathbf{g}}_\lambda]^T  \mathbf{F}_{\lambda} (\lambda_0)  \hat{\mathbf{g}}_\lambda = \| \hat{\mathbf{g}}_\lambda \|^2_{F_{\lambda_0}}
\end{aligned}\tag{9}\label{9}
$$`



# Riemannian Steepest Direction is Invariant
------
Now, we can show that the optimal solution of [Riemannian steepest direction]({{ site.baseurl }}{% post_url 2021-10-04-Geomopt02 %}#riemannian-steepest-direction) considered in Part II  under parametrization $\tau$ and $\lambda$ are equivalent since both the length and the directional derivative remain the same.

Denote Euclidean gradients as `$\mathbf{g}_\lambda:= \nabla  f_\lambda(\mathbf{\lambda}_0) $` and  `$\mathbf{g}_\tau:= \nabla  f_\tau(\mathbf{\tau}_0)  = \nabla  f_\lambda(\mathbf{\lambda}(\tau_0)) $`, which follows the parameter transformation rule in  `$\eqref{6}$`.
 

Now, consider natural/Riemannian gradients as `$\hat{\mathbf{g}}_\lambda:= \mathbf{F}_{\lambda}^{-1}(\mathbf{\lambda}_0)  \mathbf{g}_\lambda $` and  `$\hat{\mathbf{g}}_\tau:= \mathbf{F}_{\tau}^{-1}(\mathbf{\tau}_0) \mathbf{g}_\tau $`. These Riemannian gradients follow the parameter transformation rule in `$\eqref{7}$` as shown below.

`$$
\begin{aligned}
\hat{\mathbf{g}}_\tau &= \mathbf{F}_{\tau}^{-1}(\mathbf{\tau}_0) \mathbf{g}_\tau \\
&= \big( \mathbf{J}^T  \mathbf{F}_{\lambda} (\mathbf{\lambda}_0) \mathbf{J} \big)^{-1} ( \mathbf{g}^T_\tau )^T & ( \text{by } \eqref{8} )\\
&=  \mathbf{J}^{-1} \mathbf{F}_{\lambda}^{-1} (\mathbf{\lambda}_0) \mathbf{J}^{-T}   ( \mathbf{g}^T_\lambda \mathbf{J} )^T  & ( \text{by } \eqref{6} ) \\
&=  \mathbf{J}^{-1} \mathbf{F}_{\lambda}^{-1} (\mathbf{\lambda}_0) \mathbf{J}^{-T}  (  \mathbf{J}^T  \mathbf{g}_\lambda  ) \\
&=  \mathbf{J}^{-1} \mathbf{F}_{\lambda}^{-1} (\mathbf{\lambda}_0)   \mathbf{g}_\lambda   \\
&=  \mathbf{J}^{-1}   \hat{\mathbf{g}}_\lambda
\end{aligned}
$$`

Recall that the optimal solution of the Riemannian steepest direction is
`$$
\begin{aligned}
\mathbf{v}_{\lambda}^{(opt)}= -\frac{ \mathbf{F_\lambda}^{-1}(\mathbf{\lambda}_0) \nabla_\lambda f(\mathbf{\lambda}_0) }{\| \mathbf{F_\lambda}^{-1}(\mathbf{\lambda}_0)\nabla_\lambda f(\mathbf{\lambda}_0) \|_{F_{\lambda_0}}} = -\frac{\hat{\mathbf{g}}_\lambda}{\|\hat{\mathbf{g}}_\lambda\|_{ F_{\lambda_0} } } \\
\mathbf{v}_{\tau}^{(opt)}= -\frac{ \mathbf{F_\tau}^{-1}(\mathbf{\tau}_0) \nabla_\tau f(\mathbf{\tau}_0) }{\| \mathbf{F_\tau}^{-1}(\mathbf{\tau}_0)\nabla_\tau f(\mathbf{\tau}_0) \|_{F_{\tau_0}}} = -\frac{\hat{\mathbf{g}}_\tau}{\|\hat{\mathbf{g}}_\tau\|_{ F_{\tau_0} } } 
\end{aligned}
$$`
 
We can easily verify the following identities since
`$ \|\hat{\mathbf{g}}_\lambda\|_{ F_{\lambda_0} } =  \|\hat{\mathbf{g}}_\tau\|_{ F_{\tau_0} }  $` as shown in `$\eqref{9}$`.
`$$
\begin{aligned}
\mathbf{g}_\tau^T   \mathbf{v}^{(opt)}_{\tau}   & =   \mathbf{g}_\lambda^T  \mathbf{v}^{(opt)}_{\lambda} & \,\,\, \text{(invariance of a directional derivative)}  \\
\|  \mathbf{v}^{(opt)}_{\tau} \|^2_{\color{red}{F_{\tau_0}}} & = \|  \mathbf{v}^{(opt)}_{\lambda} \|^2_{\color{red}{F_{\lambda_0}} } & \,\,\, \text{(invariance of the length of the Riemannian steepest direction)}  \\
\mathbf{v}^{(opt)}_{\tau} & = \mathbf{J}^{-1}  \mathbf{v}^{(opt)}_{\lambda} & \,\,\, \text{(transformation rule for the Riemannian steepest direction)}  
\end{aligned}.
$$` 
In other words, the Riemannian steepest direction (which is indeed  a normalized Riemannian gradient) is also transformed according to the transformation rule for Riemannian gradients in `$\eqref{7}$`.

As we will discuss in [Part IV]({{ site.baseurl }}{% post_url 2021-11-15-Geomopt04 %}#natural-gradient-descent-is-linearly-invariant), this invariance property implies that natural-gradient descent is linearly invariant.
 




# Euclidean Steepest Direction is NOT Invariant
------
Recall that we have shown that a Euclidean gradient is the optimal solution of  [Euclidean steepest direction]({{ site.baseurl }}{% post_url 2021-10-04-Geomopt02 %}#euclidean-steepest-direction-and directional-derivative) in Part II.

 

We can show that the (standard) length of a Euclidean gradient is NOT invariant under a parameter transformation due to the Jacobian matrix (i.e., `$\| \mathbf{g}_\tau \| \neq \| \mathbf{g}_\lambda \|$`). This is a reason why we use the [weighted inner product]({{ site.baseurl }}{% post_url 2021-10-04-Geomopt02 %}#distance-induced-by-the-fisher-rao-metric) to define the length of a gradient vector.

Note that we denote the Euclidean gradients as `$\mathbf{g}_\lambda:= \nabla  f_\lambda(\mathbf{\lambda}_0) $` and  `$\mathbf{g}_\tau:= \nabla  f_\tau(\mathbf{\tau}_0)  = \nabla  f_\lambda(\mathbf{\lambda}(\tau_0)) $`


Recall that the optimal solution of the [Euclidean steepest direction]({{ site.baseurl }}{% post_url 2021-10-04-Geomopt02 %}#euclidean-steepest-direction-and-directional-derivative) is
`$$
\begin{aligned}
\mathbf{v}_{\lambda}^{(opt)}= -\frac{\nabla_\lambda f_\lambda(\mathbf{\lambda}_0) }{\|\nabla_\lambda f_\lambda(\mathbf{\lambda}_0)  \|} = -\frac{\mathbf{g}_\lambda}{\|\mathbf{g}_\lambda\|} \\
\mathbf{v}_{\tau}^{(opt)}= -\frac{\nabla_\tau f_\tau(\mathbf{\tau}_0) }{\|\nabla_\tau f_{\tau}(\mathbf{\tau}_0) \|} = -\frac{\mathbf{g}_\tau}{\|\mathbf{g}_\tau\|} 
\end{aligned}
$$`

Unfortunately, the Euclidean steepest direction  does NOT obey the parameter transformation rule for Euclidean gradients in  `$\eqref{6}$`.
`$$
\begin{aligned}
(\mathbf{v}_{\tau}^{(opt)})^T \neq (\mathbf{v}_{\lambda}^{(opt)})^T \mathbf{J} 
\end{aligned}
$$`


Moreover, the optimal value of the Euclidean steepest direction is NOT invariant under a parameter transformation as
`$$
\begin{aligned}
\mathbf{g}_\lambda^T \mathbf{v}^{(opt)}_{\lambda}  = - \|\mathbf{g}_\lambda\| \neq - \|\mathbf{g}_\tau\| = \mathbf{g}_\tau^T \mathbf{v}^{(opt)}_{\tau} 
\end{aligned}
$$`  

In summary, the Euclidean steepest direction (which is a normalized Euclidean gradient) is NOT transformed according to the transformation rule for a Euclidean gradient.
Moreover, Euclidean gradient descent is not invariant under a parameter transformation. We will cover more about this in [Part IV]({{ site.baseurl }}{% post_url 2021-11-15-Geomopt04 %})





------
# References
{% bibliography --cited %}

## Footnotes:
[^1]: In differential geometry, a Euclidean gradient is also known as a coordinate representation of a cotangent vector.

[^2]: We assume readers are familar with the transformation rule for Euclidean gradients. In differential geometry, this transformation rule can also be shown by using an abstract coordinate map. We avoid defining this map for simplicity.


